cava/Cava/Monad/SequentialTimed.v
@@ -1,0 +1,196 @@
+(****************************************************************************)
+(* Copyright 2020 The Project Oak Authors                                   *)
+(*                                                                          *)
+(* Licensed under the Apache License, Version 2.0 (the "License")           *)
+(* you may not use this file except in compliance with the License.         *)
+(* You may obtain a copy of the License at                                  *)
+(*                                                                          *)
+(*     http://www.apache.org/licenses/LICENSE-2.0                           *)
+(*                                                                          *)
+(* Unless required by applicable law or agreed to in writing, software      *)
+(* distributed under the License is distributed on an "AS IS" BASIS,        *)
+(* WITHOUT WARRANTIES OR CONDITIONS OF ANY KIND, either express or implied. *)
+(* See the License for the specific language governing permissions and      *)
+(* limitations under the License.                                           *)
+(****************************************************************************)
+
+From Coq Require Import Bool.Bool.
+From Coq Require Import Strings.Ascii Strings.String.
+Require Import ExtLib.Structures.Monads.
+Require Export ExtLib.Data.Monads.IdentityMonad.
+Require Import ExtLib.Structures.Traversable.
+Export MonadNotation.
+
+Require Import Coq.Vectors.Vector.
+Require Import Coq.Bool.Bvector.
+Import VectorNotations.
+
+From Coq Require Import Fin.
+From Coq Require Import NArith.Ndigits.
+From Coq Require Import ZArith.ZArith.
+
+From Coq Require Import micromega.Lia.
+
+Require Import Cava.Cava.
+From Cava Require Import Kind.
+From Cava Require Import Signal.
+Require Import Cava.Monad.CavaClass.
+Require Import Cava.Monad.TimedMonad.
+Require Import Cava.Monad.CombinationalMonad.
+
+(******************************************************************************)
+(* Delay combinator.                                                          *)
+(******************************************************************************)
+
+Definition delay {A} (x : timed (combType A)) : timed (combType A) :=
+  fun t =>
+    match t with
+    | 0 => defaultCombValue A
+    | S t' => x t'
+    end.
+
+(******************************************************************************)
+(* Loop combinator for feedback with delay.                                   *)
+(******************************************************************************)
+
+Definition loopSeqF' {A B C : SignalType}
+         (f : combType A * combType C -> combType B * combType C)
+         (a : timed (combType A)) : timed (combType B * combType C) :=
+  timedFold (fun bc a => f (a, snd bc)) (defaultCombValue B, defaultCombValue C) a.
+
+Definition loopSeqF {A B C : SignalType}
+         (f : combType A * combType C -> timed (combType B * combType C))
+         (a : timed (combType A)) : timed (combType B) :=
+  '(b, _) <- loopSeqF' (fun ac => f ac 0) a ;;
+  ret b.
+
+(******************************************************************************)
+(* A boolean sequential logic interpretation for the Cava class               *)
+(******************************************************************************)
+
+Definition unopF (f : bool -> bool) (i : combType Bit) : timed (combType Bit) :=
+  ret (f i).
+
+Definition binopF (f : bool -> bool -> bool) (i : combType Bit * combType Bit) : timed (combType Bit) :=
+  ret (f (fst i) (snd i)).
+
+Definition lut1BoolF (f: bool -> bool) (i : bool) : timed bool :=
+  ret (f i).
+
+Definition lut2BoolF (f: bool -> bool -> bool) (i : bool * bool) : timed bool :=
+  let '(i0, i1) := i in
+  ret (f i0 i1).
+
+Definition lut3BoolF (f: bool -> bool -> bool -> bool) (i : bool * bool * bool) : timed bool :=
+  let '(i0, i1, i2) := i in
+  ret (f i0 i1 i2).
+
+Definition lut4BoolF (f: bool -> bool -> bool -> bool -> bool) (i : bool * bool * bool * bool) : timed bool :=
+  let '(i0, i1, i2, i3) := i in
+  ret (f i0 i1 i2 i3).
+
+Definition lut5BoolF (f: bool -> bool -> bool -> bool -> bool -> bool)
+           (i : bool * bool * bool * bool * bool) : timed bool :=
+  let '(i0, i1, i2, i3, i4) := i in
+  ret (f i0 i1 i2 i3 i4).
+
+Definition lut6BoolF (f: bool -> bool -> bool -> bool -> bool -> bool -> bool)
+           (i : bool * bool * bool * bool * bool * bool) : timed bool :=
+  let '(i0, i1, i2, i3, i4, i5) := i in
+  ret (f i0 i1 i2 i3 i4 i5).
+
+Definition muxcyBoolF (s ci di : bool) : timed bool :=
+  ret (if s then ci else di).
+
+Local Open Scope list_scope.
+
+Definition unsignedAddComb {m n : nat}
+                           (av : Bvector m) (bv : Bvector n) :
+                           Bvector (1 + max m n) :=
+  let a := Bv2N av in
+  let b := Bv2N bv in
+  let sumSize := 1 + max m n in
+  let sum := (a + b)%N in
+  N2Bv_sized sumSize sum.
+
+Definition unsignedAddBoolF {m n : nat} (av : Bvector m) (bv : Bvector n)
+  : timed (Bvector (1 + max m n)) :=
+  ret (unsignedAddComb av bv).
+
+Definition unsignedMultComb {m n : nat}
+           (av : Bvector m) (bv : Bvector n)
+  : Bvector (m + n) :=
+  let a := Bv2N av in
+  let b := Bv2N bv in
+  let product := (a * b)%N in
+  N2Bv_sized (m + n) product.
+
+Definition unsignedMultBoolF {m n : nat} (av : Bvector m) (bv : Bvector n)
+  : timed (Bvector (m + n)) :=
+  ret (unsignedMultComb av bv).
+
+Definition greaterThanOrEqualComb
+           {m n : nat} (av : Bvector m) (bv : Bvector n) : bool :=
+  let a := N.to_nat (Bv2N av) in
+  let b := N.to_nat (Bv2N bv) in
+  b <=? a.
+
+Definition greaterThanOrEqualBoolF {m n : nat} (av : Bvector m) (bv : Bvector n)
+  : timed bool :=
+  ret (greaterThanOrEqualComb av bv).
+
+
+Definition blackBoxF (intf : CircuitInterface)
+  : timed (tupleInterface combType (List.map port_type (circuitOutputs intf))) :=
+  ret (tupleInterfaceDefault (map port_type (circuitOutputs intf))).
+
+
+(******************************************************************************)
+(* Instantiate the Cava class for a boolean sequential logic                  *)
+(* interpretation.                                                            *)
+(******************************************************************************)
+
+ Instance TimedCombSemantics : Cava combType :=
+  { cava := timed;
+    zero := ret false;
+    one := ret true;
+    defaultSignal t := defaultCombValue t;
+    inv := unopF negb;
+    and2 := binopF andb;
+    nand2 := binopF (fun a b => negb (andb a b));
+    or2 := binopF orb;
+    nor2 := binopF (fun a b => negb (orb a b));
+    xor2 := binopF xorb;
+    xnor2 := binopF (fun a b => negb (xorb a b));
+    buf_gate := @ret timed Monad_timed bool;
+    lut1 := lut1BoolF;
+    lut2 := lut2BoolF;
+    lut3 := lut3BoolF;
+    lut4 := lut4BoolF;
+    lut5 := lut5BoolF;
+    lut6 := lut6BoolF;
+    xorcy := binopF xorb;
+    muxcy := muxcyBoolF;
+    peel _ _ v := v;
+    unpeel _ _ v := v;
+    indexAt t sz isz := @indexAtBool t sz isz;
+    indexConst t sz := @indexConstBool t sz;
+    slice t sz := @sliceBool t sz;
+    unsignedAdd m n := @unsignedAddBoolF m n;
+    unsignedMult m n := @unsignedMultBoolF m n;
+    greaterThanOrEqual m n := @greaterThanOrEqualBoolF m n;
+    instantiate _ circuit := circuit;
+    blackBox intf _ := blackBoxF intf;
+  }.
+
+ Instance TimedSeqSemantics : CavaSeqMonad TimedCombSemantics :=
+   { delaym k i := delay i;
+     loopm A B C := @loopSeqF A B C;
+   }.
+
+(******************************************************************************)
+(* A function to run a monadic circuit description and return the boolean     *)
+(* behavioural simulation result at the given timestep.                       *)
+(******************************************************************************)
+
+Definition sequentialF {a} (circuit : cava a) (t : nat) : a := circuit t.
