cava/Cava/Monad/TimedMonad.v
@@ -1,0 +1,118 @@
+(****************************************************************************)
+(* Copyright 2020 The Project Oak Authors                                   *)
+(*                                                                          *)
+(* Licensed under the Apache License, Version 2.0 (the "License")           *)
+(* you may not use this file except in compliance with the License.         *)
+(* You may obtain a copy of the License at                                  *)
+(*                                                                          *)
+(*     http://www.apache.org/licenses/LICENSE-2.0                           *)
+(*                                                                          *)
+(* Unless required by applicable law or agreed to in writing, software      *)
+(* distributed under the License is distributed on an "AS IS" BASIS,        *)
+(* WITHOUT WARRANTIES OR CONDITIONS OF ANY KIND, either express or implied. *)
+(* See the License for the specific language governing permissions and      *)
+(* limitations under the License.                                           *)
+(****************************************************************************)
+
+Require Import Coq.Arith.PeanoNat.
+Require Import Coq.Lists.List.
+Require Import ExtLib.Structures.Monads.
+Import ListNotations.
+Import MonadNotation.
+Local Open Scope monad_scope.
+
+(**** Monad representing an infinite stream of values ****)
+
+Definition timed (A : Type) : Type := nat -> A.
+
+Instance Monad_timed : Monad timed :=
+  {| ret := fun _ x t => x;
+     bind :=
+       fun A B (x : timed A) (f : A -> timed B) t =>
+         f (x t) t
+  |}.
+
+Definition asList {A} (x : timed A) (n : nat) := List.map x (seq 0 n).
+
+(* Create a timed monad from a start state and step function *)
+Definition timedFix {A} (f : A -> A) (x : A) : timed A :=
+  fix body (t : nat) :=
+    match t with
+    | 0 => x
+    | S t' => f (body t')
+    end.
+
+(* Stateful version of timedFix; given a start state and a timed input, loop a
+   function over state and input to produce a timed output. *)
+Definition timedFold {A B} (f : A -> B -> A) (x : A) (y : timed B) : timed A :=
+  fix body (t : nat) :=
+    match t with
+    | 0 => x
+    | S t' => f (body t') (y t')
+    end.
+
+Section Examples.
+  (* Simple timed definition that returns the timestep *)
+  Let countUp : timed nat := fun t => t.
+
+  (* If we compute the first five results of countUp, we should get 0...4 *)
+  Goal (asList countUp 5 = [0;1;2;3;4]).
+  Proof. reflexivity. Qed.
+
+  (* Multiplication *)
+  Let multiply (x y : nat) : timed nat := ret (x * y).
+
+  (* If we multiply two countUps, we should get a list of squares *)
+  Goal (asList (x <- countUp ;;
+                y <- countUp ;;
+                multiply x y) 5 = [0;1;4;9;16]).
+  Proof. vm_compute. reflexivity. Qed.
+
+  (* Delays the input stream one step *)
+  Let delayNat (x : timed nat) : timed nat :=
+    fun t =>
+      match t with
+      | 0 => 0
+      | S t' => x t'
+      end.
+
+  (* If we delay one of the countUps, we should get 0*0, 0*1, 1*2, 2*3, 3*4 *)
+  Goal (asList
+          (x <- delayNat countUp ;;
+           y <- countUp ;;
+           multiply x y) 5 = [0;0;2;6;12]).
+  Proof. vm_compute. reflexivity. Qed.
+
+  (* If we delay both inputs to multiply, we should get the list of squares but
+     delayed one step. *)
+  Goal (asList
+          (x <- delayNat countUp ;;
+           y <- delayNat countUp ;;
+           multiply x y) 5 = [0;0;1;4;9]).
+  Proof. vm_compute. reflexivity. Qed.
+
+  (* counter that increments state by 1 each timestep *)
+  Let counter : timed nat := timedFix (Nat.add 1) 0.
+
+  Goal (asList counter 5 = [0;1;2;3;4]).
+  Proof. vm_compute. reflexivity. Qed.
+
+  (* counter that adds the input to the state *)
+  Let countBy : timed nat -> timed nat := timedFold Nat.add 0.
+
+  Goal (asList (countBy countUp) 10 = [0;0;1;3;6;10;15;21;28;36]).
+  Proof. vm_compute. reflexivity. Qed.
+
+End Examples.
+
+Section Proofs.
+  Lemma timedFold_fold_left {A B} (f : A -> B -> A) a bs t :
+    (timedFold f a bs) t = fold_left f (asList bs t) a.
+  Proof.
+    cbv [asList].
+    revert t a bs; induction t; [ reflexivity | ].
+    intros. cbn [timedFold]. rewrite seq_S.
+    rewrite map_app, fold_left_app. cbn [fold_left map].
+    rewrite IHt; reflexivity.
+  Qed.
+End Proofs.
